ALterações no projeto

proj1/proj1.dfy
@@ -10,7 +10,7 @@ requires 0 <= i <= j <= a.Length
 }
 
 method query (a:array<int>, i:int, j:int) returns (s:int)
-requires 0 <= i <= j < a.Length
+requires 0 <= i <= j <= a.Length
 ensures s == sum(a, i, j)
 {
     s := 0;
@@ -27,34 +27,49 @@ ensures s == sum(a, i, j)
     return s;
 }
 
-
+lemma queryLemma(a:array<int>, i:int, j:int, k:int)
+    requires 0 <= i <= j <= a.Length
+    requires 0 <= i <= k <= j <= a.Length
+    ensures  sum(a,i,k) + sum(a,k,j) == sum(a,i,j)
+{
+}
 
 
 
 method queryFast (a:array<int>, c:array<int>, i:int, j:int) returns (r:int)
-requires is_prefix_sum_for(a,c) ∧ 0 <= i <= j <= a.Length ∧ a.Length < c.Length
+requires is_prefix_sum_for(a,c) && 0 <= i <= j <= a.Length && a.Length < c.Length
+ensures r == sum(a, i,j)
 {
-    r:= 0;
+    r := c[j] - c[i];
+    queryLemma(a,0,j,i);
 
-    if i == 0{
-        r := c[j - 1];
-    }
-    else {
-        r := c[j-1] - c[i-1];
-    }
     return r;
 }
 
 predicate is_prefix_sum_for (a:array<int>, c:array<int>)
 reads c, a
 {
-    var i := c.Length;
+    a.Length + 1 == c.Length
+    && c[0] == 0
+    && forall j :: 1 <= j <= a.Length ==> c[j] == sum(a,0,j)
+}
 
-    while (i >= 1)
-    invariant 1 <= i <= c.Length
-    decreases i
+datatype List<T> = Nil | Cons(head: T, tail: List<T>)
+
+method from_array<T>(a: array<T>) returns (l: List<T>)
+requires a.Length > 0
+{
+    var i:= a.Length-1;
+
+    l:= Nil;
+
+    while (i >= 0)
+    invariant -1 <= i < a. Length
+    decreases i;
     {
-        c[i] == sum(a,0,i-1);
-        i := i - 1;
+        l := Cons(a[i], l);
+        i:= i-1;
     }
+    return l;
+
 }
